output syntax for pattern aliases

src/HOL/Library/Pattern_Aliases.thy
@@ -11,7 +11,7 @@ begin
 text \<open>
   Most functional languages (Haskell, ML, Scala) support aliases in patterns. This allows to refer
   to a subpattern with a variable name. This theory implements this using a check phase. It works
-  well for function definitions (see usage below).
+  well for function definitions (see usage below). All features are packed into a @{command bundle}.
 
   The following caveats should be kept in mind:
   \<^item> The translation expects a term of the form @{prop "f x y = rhs"}, where \<open>x\<close> and \<open>y\<close> are patterns
@@ -22,8 +22,10 @@ text \<open>
   \<^item> Terms that do not adhere to the above shape may either stay untranslated or produce an error
     message. The @{command fun} command will complain if pattern aliases are left untranslated.
     In particular, there are no checks whether the patterns are wellformed or linear.
-  \<^item> There is no corresonding uncheck phase, because it is unclear in which situations the
-    translation should be reversed.
+  \<^item> The corresponding uncheck phase attempts to reverse the translation (no guarantee).
+  \<^item> To obtain reasonable induction principles in function definitions, the bundle also declares
+    a custom congruence rule for @{const Let} that only affects @{command fun}. This congruence
+    rule might lead to an explosion in term size (although that is rare)!
 \<close>
 
 
@@ -31,10 +33,14 @@ subsection \<open>Definition\<close>
 
 consts as :: "'a \<Rightarrow> 'a \<Rightarrow> 'a"
 
+lemma let_cong_unfolding: "M = N \<Longrightarrow> f N = g N \<Longrightarrow> Let M f = Let N g"
+by simp
+
 ML\<open>
 local
 
 fun let_typ a b = a --> (a --> b) --> b
+fun as_typ a = a --> a --> a
 
 fun strip_all t =
   case try Logic.dest_all t of
@@ -43,6 +49,27 @@ fun strip_all t =
 
 fun all_Frees t =
   fold_aterms (fn Free (x, t) => insert op = (x, t) | _ => I) t []
+
+fun subst_once (old, new) t =
+  let
+    fun go t =
+      if t = old then
+        (new, true)
+      else
+        case t of
+          u $ v =>
+            let
+              val (u', substituted) = go u
+            in
+              if substituted then
+                (u' $ v, true)
+              else
+                case go v of (v', substituted) => (u $ v', substituted)
+            end
+        | Abs (name, typ, t) =>
+            (case go t of (t', substituted) => (Abs (name, typ, t'), substituted))
+        | _ => (t, false)
+  in fst (go t) end
 
 in
 
@@ -53,7 +80,7 @@ fun check_pattern_syntax t =
         fun go (Const (@{const_name as}, _) $ pat $ var, rhs) =
               let
                 val (pat', rhs') = go (pat, rhs)
-                val _ = if is_Free var then () else error "Left-hand side of =: must be a free variable"
+                val _ = if is_Free var then () else error "Right-hand side of =: must be a free variable"
                 val rhs'' =
                   Const (@{const_name Let}, let_typ (fastype_of var) (fastype_of rhs)) $
                     pat' $ lambda var rhs'
@@ -75,6 +102,35 @@ fun check_pattern_syntax t =
       in fold (fn v => Logic.dependent_all_name ("", v)) (map Free frees) res end
   | _ => t
 
+fun uncheck_pattern_syntax ctxt t =
+  case strip_all t of
+    (vars, @{const Trueprop} $ (Const (@{const_name HOL.eq}, _) $ lhs $ rhs)) =>
+      let
+        fun go lhs (rhs as Const (@{const_name Let}, _) $ pat $ Abs (name, typ, t)) ctxt frees =
+              if exists_subterm (fn t' => t' = pat) lhs then
+                let
+                  val ([name'], ctxt') = Variable.variant_fixes [name] ctxt
+                  val free = Free (name', typ)
+                  val subst = (pat, Const (@{const_name as}, as_typ typ) $ pat $ free)
+                  val lhs' = subst_once subst lhs
+                  val rhs' = subst_bound (free, t)
+                in
+                  go lhs' rhs' ctxt' (Free (name', typ) :: frees)
+                end
+              else
+                (lhs, rhs, ctxt, frees)
+          | go lhs rhs ctxt frees = (lhs, rhs, ctxt, frees)
+
+        val (lhs', rhs', _, frees) = go lhs rhs ctxt []
+
+        val res =
+          HOLogic.mk_Trueprop (HOLogic.mk_eq (lhs', rhs'))
+          |> fold (fn v => Logic.dependent_all_name ("", v)) (map Free vars @ frees)
+      in
+        if null frees then t else res
+      end
+  | _ => t
+
 end
 \<close>
 
@@ -83,6 +139,9 @@ bundle pattern_aliases begin
   notation as (infixr "=:" 1)
 
   declaration \<open>K (Syntax_Phases.term_check 98 "pattern_syntax" (K (map check_pattern_syntax)))\<close>
+  declaration \<open>K (Syntax_Phases.term_uncheck 98 "pattern_syntax" (map o uncheck_pattern_syntax))\<close>
+
+  declare let_cong_unfolding [fundef_cong]
 
 end
 
@@ -103,11 +162,22 @@ by (rule test_1_def[unfolded Let_def])
 text \<open>Very useful for function definitions.\<close>
 
 private fun test_2 where
-"test_2 (y # (y' # ys =: x') =: x) = x @ x'" |
+"test_2 (y # (y' # ys =: x') =: x) = x @ x' @ x'" |
 "test_2 _ = []"
 
-lemma "test_2 (y # y' # ys) = (y # y' # ys) @ y' # ys"
+lemma "test_2 (y # y' # ys) = (y # y' # ys) @ (y' # ys) @ (y' # ys)"
 by (rule test_2.simps[unfolded Let_def])
+
+ML\<open>
+let
+  val actual =
+    @{thm test_2.simps(1)}
+    |> Thm.prop_of
+    |> Syntax.string_of_term @{context}
+    |> YXML.content_of
+  val expected = "\<And>x x'. test_2 (?y # (?y' # ?ys =: x') =: x) = x @ x' @ x'"
+in @{assert} (actual = expected) end
+\<close>
 
 end
 
